- Util/Relation/SN: inductive definition of strong normalization   (inverse of Coq accessibility) - Util/Relation/RelUtil: practical notations and useful results   on composition, union and reflexive and transitive closures - Term/WithArity: elimination of useless hypotheses   in AWFMInterpretation and ARedOrd - Util/Relation/Lexico: new formalization of lexicographic ordering   with minimal hypotheses - Term/WithArity/ATrs: rewriting modulo the transitive closure of some relation - Term/WithArity/ARedOrd: proof of a modularity result

trunk/color/Term/WithArity/ARelation.v
@@ -7,7 +7,7 @@ See the COPYRIGHTS and LICENSE files.
 general definitions and results about relations on terms
 ************************************************************************)
 
-(* $Id: ARelation.v,v 1.5 2006-10-26 14:26:06 blanqui Exp $ *)
+(* $Id: ARelation.v,v 1.6 2006-12-01 09:37:48 blanqui Exp $ *)
 
 Set Implicit Arguments.
 
@@ -20,6 +20,8 @@ Variable Sig : Signature.
 Require Export ATrs.
 
 Notation term := (term Sig).
+Notation rule := (rule Sig).
+Notation rules := (list rule).
 
 Require Export ASubstitution.
 
@@ -38,45 +40,60 @@ Definition context_closed :=
 
 Definition rewrite_ordering := substitution_closed /\ context_closed.
 
-Require Export WfUtil.
+Require Export SN.
 
-Definition reduction_ordering := wf succ /\ rewrite_ordering.
+Definition reduction_ordering := WF succ /\ rewrite_ordering.
 
 (***********************************************************************)
 (* compatibility *)
 
-Definition compatible R := forall l r : term, In (mkRule l r) R -> succ l r.
+Variable R : rules.
 
-Lemma comp_rewrite_ord : forall R, rewrite_ordering -> compatible R ->
+Definition compatible := forall l r : term, In (mkRule l r) R -> succ l r.
+
+Lemma comp_rewrite_ord : rewrite_ordering -> compatible ->
   forall t u, red R t u -> succ t u.
 
 Proof.
-intros R (Hsubs,Hcont) Hcomp t u H. redtac. subst t. subst u.
+intros (Hsubs,Hcont) Hcomp t u H. redtac. subst t. subst u.
 apply Hcont. apply Hsubs. apply Hcomp. exact H.
 Qed.
 
-Lemma comp_rewrite_ord_incl : forall R, rewrite_ordering -> compatible R ->
-  inclusion (red R) succ.
+Lemma comp_rewrite_ord_incl : rewrite_ordering -> compatible -> red R << succ.
 
 Proof.
-unfold inclusion. intros. apply comp_rewrite_ord with (R := R); assumption.
+unfold inclusion. intros. apply comp_rewrite_ord; assumption.
 Qed.
 
-Lemma comp_head_rewrite_ord : forall R, substitution_closed -> compatible R ->
+Lemma comp_head_rewrite_ord : substitution_closed -> compatible ->
   forall t u, hd_red R t u -> succ t u.
 
 Proof.
 intros. redtac. subst t. subst u. apply H. apply H0. assumption.
 Qed.
 
-Lemma comp_head_rewrite_ord_incl : forall R, substitution_closed ->
-  compatible R -> inclusion (hd_red R) succ.
+Lemma comp_head_rewrite_ord_incl :
+  substitution_closed -> compatible -> hd_red R << succ.
 
 Proof.
-unfold inclusion. intros. apply comp_head_rewrite_ord with (R := R); assumption.
+unfold inclusion. intros. apply comp_head_rewrite_ord; assumption.
 Qed.
 
 End basic.
+
+Lemma comp_mod_rewrite_ord_incl : forall succ R E,
+  rewrite_ordering succ -> compatible succ E -> compatible succ R ->
+  red_mod E R << succ!.
+
+Proof.
+unfold inclusion. intros. do 2 destruct H2. deduce (rtc_split H2). destruct H4.
+subst x0. apply t_step. apply incl_elim with (R := red R). 2: exact H3.
+apply comp_rewrite_ord_incl; assumption.
+apply t_trans with (y := x0). apply incl_elim with (R := red E !).
+2: exact H4. apply incl_tc. apply comp_rewrite_ord_incl; assumption.
+apply t_step. apply incl_elim with (R := red R). 2: exact H3.
+apply comp_rewrite_ord_incl; assumption.
+Qed.
 
 Record Rewrite_ordering : Type := mkRewrite_ordering {
   rew_ord_rel :> relation term;
@@ -105,7 +122,7 @@ Definition weak_context_closed :=
 Definition weak_rewrite_ordering :=
   substitution_closed succ /\ weak_context_closed.
 
-Definition weak_reduction_ordering := wf succ /\ weak_rewrite_ordering.
+Definition weak_reduction_ordering := WF succ /\ weak_rewrite_ordering.
 
 (***********************************************************************)
 (* reduction pairs *)
@@ -117,15 +134,55 @@ Definition reduction_pair :=
 
 End reduction_pair.
 
+Record Weak_reduction_pair : Type := mkWeak_reduction_pair {
+  wp_succ : relation term;
+  wp_succ_eq : relation term;
+  wp_subs : substitution_closed wp_succ;
+  wp_subs_eq : substitution_closed wp_succ_eq;
+  wp_cont : weak_context_closed wp_succ wp_succ_eq;
+  wp_cont_eq : context_closed wp_succ_eq;
+  wp_comp : inclusion (compose wp_succ_eq wp_succ) wp_succ;
+  wp_succ_wf : WF wp_succ
+}.
+
 Record Reduction_pair : Type := mkReduction_pair {
   rp_succ : relation term;
   rp_succ_eq : relation term;
   rp_subs : substitution_closed rp_succ;
   rp_subs_eq : substitution_closed rp_succ_eq;
-  rp_cont : weak_context_closed rp_succ rp_succ_eq;
+  rp_cont : context_closed rp_succ;
   rp_cont_eq : context_closed rp_succ_eq;
-  rp_comp : inclusion (compose rp_succ_eq rp_succ) rp_succ
+  rp_comp : inclusion (compose rp_succ_eq rp_succ) rp_succ;
+  rp_succ_wf : WF rp_succ
 }.
+
+(***********************************************************************)
+(* union of rewrite rules *)
+
+Section union.
+
+Variables R R' : rules.
+
+Lemma red_union : red (R ++ R') << red R U red R'.
+
+Proof.
+unfold inclusion. intros. redtac. subst x. subst y.
+deduce (in_app_or H). destruct H0.
+left. apply red_rule. exact H0. right. apply red_rule. exact H0.
+Qed.
+
+Variables E E' : rules.
+
+Lemma red_mod_union : red_mod E (R ++ R') << red_mod E R U red_mod E R'.
+
+Proof.
+unfold inclusion. intros. do 2 destruct H. redtac. subst x0. subst y.
+deduce (in_app_or H0). destruct H1.
+left. exists (fill c (app s l)); split. assumption. apply red_rule. exact H1.
+right. exists (fill c (app s l)); split. assumption. apply red_rule. exact H1.
+Qed.
+
+End union.
 
 (***********************************************************************)
 (* reflexive closure *)
@@ -173,11 +230,33 @@ Variables (succ_eq : relation term)
 Lemma strict_left_compatible : left_compatible (strict_part succ_eq) succ_eq.
 
 Proof.
-unfold left_compatible, inclusion, compose, strict_part. intros; split; decomp H.
-eapply succ_eq_trans. apply H1. assumption.
+unfold left_compatible, inclusion, compose, strict_part.
+intros; split; decomp H. eapply succ_eq_trans. apply H1. assumption.
 unfold not; intro. deduce (succ_eq_trans H H1). contradiction.
 Qed.
 
 End strict.
 
 End S.
+
+(***********************************************************************)
+(* tactics *)
+
+Ltac destruct_rp :=
+  match goal with
+    | h : Reduction_pair _ |- _ => destruct h
+    | h : Weak_reduction_pair _ |- _ => destruct h
+    | h : reduction_ordering _ |- _ => destruct h
+    | h : rewrite_ordering _ |- _ => destruct h
+  end.
+
+Ltac WFtac := repeat destruct_rp; assumption.
+
+Ltac rptac := repeat destruct_rp; try split; assumption.
+
+Ltac incl_red :=
+  match goal with
+    | |- inclusion (red _) ?succ => apply comp_rewrite_ord_incl
+    | |- inclusion (red_mod _ _) ?succ => apply comp_mod_rewrite_ord_incl
+    | |- inclusion (hd_red _) ?succ => apply comp_head_rewrite_ord_incl
+  end; rptac.
