trunk/color/Util/Relation/Lexico.v
@@ -7,117 +7,106 @@ See the COPYRIGHTS and LICENSE files.
 lexicographic ordering
 ************************************************************************)
 
-(* $Id: Lexico.v,v 1.1 2006-10-26 14:26:06 blanqui Exp $ *)
+(* $Id: Lexico.v,v 1.2 2006-12-01 09:37:48 blanqui Exp $ *)
 
 Set Implicit Arguments.
 
-Require Export RelUtil.
+Require Export SN.
 
-Section lt_lexp.
+Section lexp.
 
-Variable (A : Set) (ltA eqA : relation A)
-  (Hcomp : inclusion (compose ltA eqA) ltA).
+Variable (A : Set) (gtA eqA : relation A) (Hcomp : eqA @ gtA << gtA).
 
-Lemma comp_Acc : forall a, Acc ltA a -> forall a', eqA a' a -> Acc ltA a'.
+Lemma SN_compat : forall a, SN gtA a -> forall a', eqA a a' -> SN gtA a'.
 
 Proof.
-intros a Acc_a a' eqa'a. apply Acc_intro. intros a'' lta''a'.
-inversion Acc_a as [H]. apply H. apply (incl_elim Hcomp). exists a'. auto.
+intros a SN_a a' eqaa'. apply SN_intro. intros a'' gta'a''.
+inversion SN_a. apply H. apply (incl_elim Hcomp). exists a'. auto.
 Qed.
 
-Variable (B : Set) (ltB : relation B).
+Variable (B : Set) (gtB : relation B).
 
 Inductive lexp : relation (prod A B) :=
-| lexp1 : forall a a' b b', ltA a' a -> lexp (a',b') (a,b)
-| lexp2 : forall a a' b b', eqA a' a -> ltB b' b -> lexp (a',b') (a,b).
+| lexp1 : forall a a' b b', gtA a a' -> lexp (a,b) (a',b')
+| lexp2 : forall a a' b b', eqA a a' -> gtB b b' -> lexp (a,b) (a',b').
 
-Variable (ltB_well_founded : well_founded ltB)
-  (eqA_trans : transitive eqA).
+Variable (gtB_WF : WF gtB) (eqA_trans : transitive eqA).
 
-Lemma lexp_Acc_eq : forall a b, Acc lexp (a,b) ->
-  forall a', eqA a' a -> Acc lexp (a',b).
+Lemma lexp_SN_eq : forall a b,
+  SN lexp (a,b) -> forall a', eqA a a' -> SN lexp (a',b).
 
 Proof.
-intros a b Acc_ab a' eqa'a. inversion Acc_ab as [H]. apply Acc_intro.
+intros a b SN_ab a' eqaa'. inversion SN_ab. apply SN_intro.
 destruct y as (a'',b'). intro H'. inversion H'; subst a'0 b'0 a0 b0; apply H.
 apply lexp1. apply (incl_elim Hcomp). exists a'. auto.
-apply lexp2. apply (eqA_trans H3 eqa'a). exact H5.
+apply lexp2. apply (eqA_trans eqaa' H4). exact H6.
 Qed.
 
-Lemma lexp_Acc :
-  forall a, Acc ltA a -> forall b, Acc ltB b -> Acc lexp (a, b).
+Lemma lexp_SN :
+  forall a, SN gtA a -> forall b, SN gtB b -> SN lexp (a, b).
 
 Proof.
-induction 1 as [a Ha1 Ha2]. induction 1 as [b Hb1 Hb2]. apply Acc_intro.
+induction 1 as [a Ha1 Ha2]. induction 1 as [b Hb1 Hb2]. apply SN_intro.
 destruct y as (a'',b'). intro H. inversion H; subst a'' b'0 a0 b0.
-(* ltA a' a *)
-apply Ha2. exact H1. apply ltB_well_founded.
-(* eqA a' a /\ ltB b' b *)
-apply (@lexp_Acc_eq a). 2: exact H3. apply Hb2. exact H5.
+(* gtA a a' *)
+apply Ha2. exact H1. apply gtB_WF.
+(* eqA a a' /\ gtB b b' *)
+apply (@lexp_SN_eq a). 2: exact H3. apply Hb2. exact H5.
 Qed.
 
-Variable ltA_well_founded : well_founded ltA.
+Variable gtA_WF : WF gtA.
 
-Lemma lexp_well_founded : well_founded lexp.
+Lemma lexp_WF : WF lexp.
 
 Proof.
-unfold well_founded. destruct a as (a,b). apply lexp_Acc.
-apply ltA_well_founded. apply ltB_well_founded.
+unfold WF. destruct x as (a,b). apply lexp_SN. apply gtA_WF. apply gtB_WF.
 Qed.
 
 Lemma lexp_intro : forall a a' b b',
-  ltA a a' \/ (eqA a a' /\ ltB b b') -> lexp (a,b) (a',b').
+  gtA a a' \/ (eqA a a' /\ gtB b b') -> lexp (a,b) (a',b').
 
 Proof.
 intros. destruct H. apply lexp1. exact H. destruct H. apply lexp2.
 exact H. exact H0.
 Qed.
 
-End lt_lexp.
+End lexp.
 
-Section gt_lexp.
-
-Require Export WfUtil.
-
-Variable (A B : Set) (gtA eqA : relation A) (gtB : relation B)
-  (eqA_trans : transitive eqA)
-  (Hcomp : inclusion (compose eqA gtA) gtA)
-  (gtA_wf : wf gtA) (gtB_wf : wf gtB).
-
-Lemma transp_lexp : inclusion (transp (lexp gtA eqA gtB))
-  (lexp (transp gtA) (transp eqA) (transp gtB)).
-
-Proof.
-unfold inclusion. destruct x as (a,b). destruct y as (a',b'). intro.
-unfold transp in H. inversion H; subst a'0 b'0 a0 b0.
-apply lexp1. exact H1. apply lexp2; auto.
-Qed.
-
-Lemma lexp_wf : wf (lexp gtA eqA gtB).
-
-Proof.
-apply (wf_incl transp_lexp). apply lexp_well_founded.
-unfold inclusion, compose, transp. intros. destruct H. destruct H.
-apply (incl_elim Hcomp). exists x0. auto. exact gtB_wf.
-apply transp_trans. apply eqA_trans. exact gtA_wf.
-Qed.
-
-End gt_lexp.
-
-Section gt_lex.
+Section lex.
 
 Variable (A : Set) (gtA eqA gtA' : relation A)
-  (eqA_trans : transitive eqA)
-  (Hcomp : inclusion (compose eqA gtA) gtA)
-  (gtA_wf : wf gtA) (gtA'_wf : wf gtA').
+  (eqA_trans : transitive eqA) (Hcomp : eqA @ gtA << gtA)
+  (gtA_WF : WF gtA) (gtA'_WF : WF gtA').
 
 Definition lex x y := lexp gtA eqA gtA' (x,x) (y,y).
 
-Lemma lex_wf : wf lex.
+Lemma lex_WF : WF lex.
 
 Proof.
-exact (wf_inv_image (fun x:A => (x,x))
-  (lexp_wf eqA_trans Hcomp gtA_wf gtA'_wf)).
+exact (WF_inverse (fun x:A => (x,x)) (lexp_WF Hcomp gtA'_WF eqA_trans gtA_WF)).
 Qed.
 
-End gt_lex.
+End lex.
+
+Section lex'.
+
+Variable (A : Set) (gt1 gt2 : relation A)
+  (gt1_WF : WF gt1) (gt2_WF : WF gt2)
+  (gt2_trans : transitive gt2) (Hcomp : gt2 @ gt1 << gt1).
+
+Definition lex' := lex gt1 gt2 gt2.
+
+Lemma lex'_WF : WF lex'.
+
+Proof.
+unfold lex'. apply lex_WF; assumption.
+Qed.
+
+Lemma lex'_intro : gt1 U gt2 << lex'.
+
+Proof.
+unfold lex', lex, inclusion. intros. apply lexp_intro. destruct H; auto.
+
+Qed.
+
+End lex'.
