trunk/color/Term/WithArity/ARedOrd.v
@@ -8,7 +8,7 @@ See the COPYRIGHTS and LICENSE files.
 termination by using compatible reduction orderings
 ************************************************************************)
 
-(* $Id: ARedOrd.v,v 1.4 2006-10-26 14:26:06 blanqui Exp $ *)
+(* $Id: ARedOrd.v,v 1.5 2006-12-01 09:37:48 blanqui Exp $ *)
 
 Set Implicit Arguments.
 
@@ -24,6 +24,8 @@ Notation term := (term Sig).
 Notation rule := (rule Sig).
 Notation rules := (list rule).
 
+Ltac WF_incl succ := apply WF_incl with (S := succ); [idtac | WFtac].
+
 (***********************************************************************)
 (* Manna-Ness theorem (1970) *)
 
@@ -31,13 +33,10 @@ Section manna_ness.
 
 Variables (R : rules) (succ : relation term).
 
-Lemma manna_ness : reduction_ordering succ -> compatible succ R -> wf (red R).
+Lemma manna_ness : reduction_ordering succ -> compatible succ R -> WF (red R).
 
 Proof.
-intros (Hwf, (Hsubst, Hcont)) Hcomp.
-apply wf_incl with (R2 := transp succ). 2: exact Hwf.
-apply incl_transp. unfold inclusion. apply comp_rewrite_ord.
-split; [exact Hsubst | exact Hcont]. exact Hcomp.
+intros. WF_incl succ. incl_red.
 Qed.
 
 End manna_ness.
@@ -48,26 +47,24 @@ several steps of R1 followed by a step of R2 *)
 
 Section manna_ness2.
 
-Variables R1 R2 : rules.
+Variables R E : rules.
 
-Let R := compose (clos_refl_trans (red R1)) (red R2).
-
-Variables (succ succ_eq : relation term)
-  (compat : inclusion (compose succ_eq succ) succ).
-
-Require Import RelUtil.
-
-Lemma manna_ness2 : reduction_ordering succ -> rewrite_ordering succ_eq
-  -> compatible succ_eq R1 -> compatible succ R2 -> wf R.
+Lemma manna_ness2_incl : forall rp : Reduction_pair Sig,
+  compatible (rp_succ_eq rp) E -> compatible (rp_succ rp) R ->
+  inclusion (red_mod E R) (rp_succ rp).
 
 Proof.
-intros (Hwf, Hsucc) Hsucceq Hcompeq Hcomp. unfold well_founded. intro.
-generalize (Hwf a). intro. elim H; clear a H. intros. apply Acc_intro. intros.
-apply H0. unfold transp. apply comp_rtc_incl_in with (R := succ_eq).
-exact compat. unfold transp, R, compose in H1. decomp H1. unfold compose.
-exists x0. split. apply incl_rtc_in with (R := red R1).
-apply comp_rewrite_ord_incl. exact Hsucceq. exact Hcompeq. exact H3.
-apply comp_rewrite_ord with (R := R2). exact Hsucc. exact Hcomp. exact H4.
+intros. unfold red_mod. apply incl_trans with
+  (S := compose (clos_refl_trans (rp_succ_eq rp)) (rp_succ rp)).
+apply incl_comp. apply incl_rtc. incl_red. incl_red.
+apply comp_rtc_incl. exact (rp_comp rp).
+Qed.
+
+Lemma manna_ness2 : forall rp : Reduction_pair Sig,
+  compatible (rp_succ_eq rp) E -> compatible (rp_succ rp) R -> WF (red_mod E R).
+
+Proof.
+intros. WF_incl (rp_succ rp). apply manna_ness2_incl; auto.
 Qed.
 
 End manna_ness2.
@@ -78,27 +75,91 @@ several steps of R1 followed by a -head- step of R2 *)
 
 Section manna_ness2_head.
 
-Variables R1 R2 : rules.
+Variables R E : rules.
 
-Let R := compose (clos_refl_trans (red R1)) (hd_red R2).
-
-Variables (succ succ_eq : relation term)
-  (compat : inclusion (compose succ_eq succ) succ).
-
-Lemma manna_ness2_head : wf succ -> substitution_closed succ
-  -> rewrite_ordering succ_eq -> compatible succ_eq R1
-  -> compatible succ R2 -> wf R.
+Lemma manna_ness2_head_incl : forall wp : Weak_reduction_pair Sig,
+  compatible (wp_succ_eq wp) E -> compatible (wp_succ wp) R ->
+  inclusion (hd_red_mod E R) (wp_succ wp).
 
 Proof.
-intros Hwf Hsucc Hsucceq Hcompeq Hcomp. unfold well_founded. intro.
-generalize (Hwf a). intro. elim H; clear a H. intros. apply Acc_intro. intros.
-apply H0. unfold transp. apply comp_rtc_incl_in with (R := succ_eq).
-exact compat. unfold transp, R, compose in H1. decomp H1. unfold compose.
-exists x0. split. apply incl_rtc_in with (R := red R1).
-apply comp_rewrite_ord_incl. exact Hsucceq. exact Hcompeq. exact H3.
-apply comp_head_rewrite_ord with (R := R2). exact Hsucc. exact Hcomp. exact H4.
+intros. unfold hd_red_mod. apply incl_trans with
+  (S := compose (clos_refl_trans (wp_succ_eq wp)) (wp_succ wp)).
+apply incl_comp. apply incl_rtc. incl_red. incl_red.
+apply comp_rtc_incl. exact (wp_comp wp).
+Qed.
+
+Lemma manna_ness2_head : forall wp : Weak_reduction_pair Sig,
+  compatible (wp_succ_eq wp) E -> compatible (wp_succ wp) R ->
+  WF (hd_red_mod E R).
+
+Proof.
+intros. WF_incl (wp_succ wp). apply manna_ness2_head_incl; auto.
 Qed.
 
 End manna_ness2_head.
+
+(***********************************************************************)
+(* rule elimination *)
+
+Section rule_elimination.
+
+Variables R R' E E' : rules.
+
+Lemma rule_elimination : forall rp : Reduction_pair Sig,
+  compatible (rp_succ_eq rp) E -> compatible (rp_succ rp) E' ->
+  compatible (rp_succ_eq rp) R -> compatible (rp_succ rp) R' ->
+  WF (red_mod E R) -> WF (red_mod (E ++ E') (R ++ R')).
+
+Proof.
+intros. set (succ := rp_succ rp). set (succ_eq := rp_succ_eq rp).
+set (er := red_mod E R). set (F := E ++ E').
+(* h0 *)
+assert (h0 : er << succ_eq!). unfold er, succ_eq. incl_red.
+(* h1 *)
+assert (h1 : red F # << succ # @ red E #).
+trans ((red E U red E')#). apply incl_rtc. unfold F. apply red_union.
+trans (red_mod E E' # @ red E #). unfold red_mod. apply rtc_union.
+comp. apply incl_rtc. unfold succ. apply manna_ness2_incl; assumption.
+(* h2 *)
+assert (h2 : red_mod F (R ++ R') << succ# @ er U succ!).
+trans (red_mod F R U red_mod F R'). apply red_mod_union. union.
+(* left *)
+unfold red_mod. trans ((succ # @ red E #) @ red R). comp. exact h1.
+trans (succ # @ (red E # @ red R)). apply comp_assoc.
+(* right *)
+trans ((succ # @ red E #) @ red R'). unfold red_mod. comp. exact h1.
+trans (succ # @ (red E # @ red R')). apply comp_assoc.
+trans (succ # @ succ). comp.
+trans (red_mod E R'). unfold succ.
+apply manna_ness2_incl; assumption. apply rtc_step_incl_tc.
+(* h3 *)
+set (gt := succ! @ succ_eq#). assert (h3 : red_mod F (R ++ R') << er U gt).
+trans (succ# @ er U succ!). exact h2.
+trans ((er U succ! @ er) U succ!). union. apply rtc_comp.
+trans (er U (succ! @ er U succ!)). apply union_assoc. union.
+trans (succ! @ er%). apply union_fact2. unfold gt. comp.
+apply incl_rc_rtc. exact h0.
+(* h4 *)
+assert (h4 : succ_eq# @ succ! << succ!).
+apply comp_incl_tc. apply comp_rtc_incl. rptac.
+(* lexico *)
+Require Import Lexico. eapply WF_incl with (S := lex' gt (er!)).
+trans (er U gt). exact h3. trans (er! U gt). union.
+apply tc_incl. trans (gt U er!). apply union_commut.
+apply lex'_intro. apply lex'_WF.
+(* WF gt *)
+unfold gt. apply WF_compat_inv. exact h4. apply WF_tc. WFtac.
+(* WF er! *)
+apply WF_tc. exact H3.
+(* er! trans *)
+apply tc_trans.
+(* compat *)
+apply comp_tc_incl. trans (succ_eq! @ gt). comp. exact h0.
+apply comp_tc_incl. unfold gt.
+trans ((succ_eq @ succ!) @ succ_eq#). apply comp_assoc'.
+comp. apply comp_incl_tc. rptac.
+Qed.
+
+End rule_elimination.
 
 End S.
